start termination proof

Earley_List.thy
@@ -60,9 +60,175 @@ definition Complete_it :: "nat \<Rightarrow> 'a item \<Rightarrow> 'a bins \<Rig
     let is = filter (\<lambda>x. next_symbol x = Some (item_rule_head y)) (items orig) in
     map (\<lambda>x. inc_item x k) is)"
 
+definition UNIV_wf_kth_bin :: "nat \<Rightarrow> 'a item set" where
+  "UNIV_wf_kth_bin k = { x | x. wf_item x \<and> item_end x = k }"
+
+definition wf_bin :: "nat \<Rightarrow> 'a bin \<Rightarrow> bool" where
+  "wf_bin k b \<longleftrightarrow> distinct (items b) \<and> (\<forall>x \<in> set (items b). wf_item x \<and> item_end x = k)"
+
+subsection \<open>Bin lemmas\<close>
+
+lemma length_bins_app_bins[simp]:
+  "length (bins (app_bins bs k is)) = length (bins bs)"
+  unfolding app_bins_def by simp
+
+lemma length_nth_bin_app_bins:
+  "length (items (bins (app_bins bs k is) ! l)) \<ge> length (items (bins bs ! l))"
+  by (cases "k < length (bins bs)") (auto simp: nth_list_update app_bins_def app_bin_def)
+
+lemma length_nth_bin_app_bins_eq:
+  "k \<noteq> l \<Longrightarrow> length (items (bins (app_bins bs k is) ! l)) = length (items (bins bs ! l))"
+  by (cases "k < length (bins bs)") (auto simp: app_bins_def app_bin_def)
+
+lemma length_bins_Init_it[simp]:
+  "length (bins Init_it) = length inp + 1"
+  unfolding Init_it_def using length_bins_app_bins by force
+
+declare set_bin_def[simp]
+
+lemma app_bins_eq:
+  "set is \<subseteq> set_bin (bins bs ! k) \<Longrightarrow> app_bins bs k is = bs"
+  using filter_False unfolding app_bins_def app_bin_def by (auto simp: in_mono)
+
+lemma nth_app_bin:
+  "i < length (items b) \<Longrightarrow> items (app_bin b is) ! i = items b ! i"
+  unfolding app_bin_def by (simp add: nth_append)
+
+lemma nth_app_bins:
+  "k \<noteq> l \<Longrightarrow> bins (app_bins bs k is) ! l = bins bs ! l"
+  unfolding app_bins_def nth_app_bin by simp
+
+lemma kth_app_bins:
+  assumes "i < length (items (bins bs ! k))"
+  shows "items (bins (app_bins bs k is) ! k) ! i = items (bins bs ! k) ! i"
+  by (cases "k < length (bins bs)") (auto simp: app_bins_def nth_app_bin assms)
+
+lemma set_bin_upto_eq_set_bin:
+  "i \<ge> length (items b) \<Longrightarrow> set_bin_upto b i = set_bin b"
+  unfolding set_bin_upto_def set_bin_def by (auto, metis in_set_conv_nth less_le_trans)
+
+lemma set_bins_upto_empty:
+  "set_bins_upto bs 0 0 = {}"
+  unfolding set_bins_upto_def set_bin_upto_def by simp
+
+lemma set_bin_app_bin[simp]:
+  "set_bin (app_bin b is) = set_bin b \<union> set is"
+  unfolding app_bin_def by auto
+
+lemma set_bins_app_bins:
+  "k < length (bins bs) \<Longrightarrow> set_bins (app_bins bs k is) = set_bins bs \<union> set is"
+  unfolding set_bins_def app_bins_def using set_bin_app_bin
+  by (auto; smt Un_iff nth_list_update_eq nth_list_update_neq set_bin_app_bin set_bin_def)+
+
+lemma kth_bin_in_bins:
+  "k < length (bins bs) \<Longrightarrow> set_bin (bins bs ! k) \<subseteq> set_bins bs"
+  unfolding set_bins_def set_bins_upto_def set_bin_upto_def by blast
+
+lemma set_bins_upto_kth_nth_id:
+  assumes "l < length (bins bs)" "k \<le> l" "i < length (items (bins bs ! k))"
+  shows "set_bins_upto (app_bins bs l is) k i = set_bins_upto bs k i"
+  unfolding set_bins_upto_def set_bin_def set_bin_upto_def app_bins_def app_bin_def
+  using assms by (auto simp: nth_append nth_list_update, metis not_less)
+
+lemma set_bins_upto_sub_set_bins:
+  "k < length (bins bs) \<Longrightarrow> set_bins_upto bs k i \<subseteq> set_bins bs"
+  unfolding set_bins_def set_bins_upto_def set_bin_upto_def using less_trans by (auto, blast)
+
+lemma set_bins_upto_Suc_Un:
+  "i < length (items (bins bs ! k)) \<Longrightarrow> set_bins_upto bs k (i+1) = set_bins_upto bs k i \<union> { items (bins bs ! k) ! i }"
+  unfolding set_bins_upto_def set_bin_upto_def using less_Suc_eq by auto
+
+lemma set_bins_upto_Suc_eq:
+  "i \<ge> length (items (bins bs ! k)) \<Longrightarrow> set_bins_upto bs k (i+1) = set_bins_upto bs k i"
+  unfolding set_bins_upto_def set_bin_upto_def by auto
+
+lemma set_bins_bin_exists:
+  "x \<in> set_bins bs \<Longrightarrow> \<exists>k < length (bins bs). x \<in> set_bin (bins bs ! k)"
+  unfolding set_bins_def by blast
+
+lemma distinct_app_bin:
+  "distinct (items b) \<Longrightarrow> distinct is \<Longrightarrow> distinct (items (app_bin b is))"
+  unfolding app_bin_def by auto
+
+lemma distinct_app_bins:
+  "distinct (items (bins bs ! k)) \<Longrightarrow> distinct is \<Longrightarrow> distinct (items (bins (app_bins bs k is) ! k))"
+  unfolding app_bins_def by (auto, metis distinct_app_bin list_update_beyond not_le_imp_less nth_list_update_eq)
+
+subsection \<open>Wellformed Bins\<close>
+
+definition wf_bins :: "'a bins \<Rightarrow> bool" where
+  "wf_bins bs \<longleftrightarrow> (\<forall>k < length (bins bs). wf_bin k (bins bs ! k))"
+
+lemma wf_bins_impl_wf_items:
+  "wf_bins bs \<Longrightarrow> wf_items (set_bins bs)"
+  unfolding wf_bins_def wf_bin_def wf_items_def set_bins_def by auto
+
+lemma wf_bins_app_bins:
+  "wf_bins bs \<Longrightarrow> distinct xs \<Longrightarrow> \<forall>x \<in> set xs. wf_item x \<and> item_end x = k \<Longrightarrow> wf_bins (app_bins bs k xs)"
+  unfolding wf_bins_def wf_bin_def app_bins_def using set_bin_app_bin distinct_app_bin
+  by (cases "k < length (bins bs)") (auto simp: nth_list_update, blast+)
+
+lemma wf_bins_kth_bin:
+  "wf_bins bs \<Longrightarrow> k < length (bins bs) \<Longrightarrow> x \<in> set_bin (bins bs ! k) \<Longrightarrow> wf_item x \<and> item_end x = k"
+  using set_bin_def wf_bin_def wf_bins_def by blast
+
+lemma wf_bins_Init_it:
+  "wf_bins Init_it"
+proof -
+  let ?rs = "filter (\<lambda>r. rule_head r = \<SS>) rules"
+  let ?b0 = "Bin (map (\<lambda>r. init_item r 0) ?rs)"
+  let ?bs = "replicate (length inp + 1) (Bin [])"
+  have "wf_bin 0 ?b0"
+    unfolding wf_bin_def wf_item_def using valid_rules by (auto simp: init_item_def distinct_map inj_on_def)
+  moreover have "wf_bins (Bins ?bs)"
+    unfolding wf_bins_def wf_bin_def using less_Suc_eq_0_disj by force
+  ultimately show ?thesis
+    using wf_bins_app_bins unfolding wf_bin_def by (simp add: Init_it_def)
+qed
+
+lemma distinct_Scan_it:
+  "distinct (Scan_it k a x)"
+  unfolding Scan_it_def by simp
+
+lemma distinct_Predict_it:
+  "distinct (Predict_it k X)"
+  unfolding Predict_it_def using valid_rules by (auto simp: init_item_def rule_head_def distinct_map inj_on_def)
+
+lemma distinct_Complete_it:
+  "wf_bins bs \<Longrightarrow> item_origin y < length (bins bs) \<Longrightarrow> distinct (Complete_it k y bs)"
+  unfolding Complete_it_def wf_bins_def wf_bin_def by (auto simp: distinct_map inj_on_def inc_item_def item.expand)
+
+lemma wf_bins_Scan_it':
+  assumes "wf_bins bs" "k < length (bins bs)" "x \<in> set_bin (bins bs ! k)"
+  assumes "k < length inp" "next_symbol x \<noteq> None" "y = inc_item x (k+1)"
+  shows "wf_item y \<and> item_end y = k+1"
+  using assms wf_bins_kth_bin[OF assms(1-3)]
+  unfolding wf_item_def inc_item_def next_symbol_def is_complete_def item_rule_body_def
+  by (auto split: if_splits)
+
+lemma wf_bins_Scan_it:
+  assumes "wf_bins bs" "k < length (bins bs)" "x \<in> set_bin (bins bs ! k)"
+  assumes "k \<le> length inp" "next_symbol x \<noteq> None"
+  shows "\<forall>y \<in> set (Scan_it k a x). wf_item y \<and> item_end y = (k+1)" 
+  using wf_bins_Scan_it'[OF assms(1-3) _ assms(5)] 
+  by (metis List.list.set(1,2) Scan_it_def empty_iff insert_iff)
+
+lemma wf_bins_Predict_it:
+  assumes "wf_bins bs" "k < length (bins bs)" "k \<le> length inp"
+  shows "\<forall>y \<in> set (Predict_it k X). wf_item y \<and> item_end y = k"
+  using assms by (auto simp: Predict_it_def wf_item_def wf_bins_def wf_bin_def init_item_def valid_rules)
+
+lemma wf_bins_Complete_it:
+  assumes "wf_bins bs" "k < length (bins bs)" "y \<in> set_bin (bins bs ! k)"
+  shows "\<forall>x \<in> set (Complete_it k y bs). wf_item x \<and> item_end x = k"
+  using assms wf_bins_kth_bin[OF assms]
+  unfolding Complete_it_def wf_bins_def wf_bin_def wf_item_def inc_item_def next_symbol_def
+            is_complete_def item_rule_body_def
+  by (auto, metis le_less_trans, metis le_less_trans le_trans)
+
 function \<pi>_it' :: "nat \<Rightarrow> 'a bins \<Rightarrow> nat \<Rightarrow> 'a bins" where
   "\<pi>_it' k bs i = (
-    if i \<ge> length (items (bins bs ! k)) then bs
+    if k \<ge> length (bins bs) \<or> \<not> wf_bins bs \<or> i \<ge> length (items (bins bs ! k)) then bs
     else
       let x = items (bins bs!k) ! i in
       let bs' =
@@ -76,7 +242,42 @@ function \<pi>_it' :: "nat \<Rightarrow> 'a bins \<Rightarrow> nat \<Rightarrow>
       in \<pi>_it' k bs' (i+1))"
   by pat_completeness simp
 termination
-  sorry
+  apply (relation "measure (\<lambda>(k,bs,i). 2 * card (UNIV_wf_kth_bin k) - card (set_bin (bins bs ! k)) - i)")
+   apply auto
+  subgoal premises prems for k bs i
+  proof -
+    show ?thesis
+      using prems apply (auto split: option.split)
+      subgoal premises prems
+      proof -
+        thm prems
+        thm distinct_card
+        find_theorems distinct app_bins
+
+        have "distinct (items (bins bs ! k))"
+          using prems(1) wf_bins_def wf_bin_def leI prems(2) by blast
+        have "item_origin (items (bins bs ! k) ! i) < length (bins bs)"
+          by (smt (verit) wf_bins_kth_bin Earley_List_def wf_defs(1) Orderings.preorder_class.dual_order.trans le_neq_implies_less linorder_linear nth_mem prems set_bin_def)
+        hence "distinct (Complete_it k (items (bins bs ! k) ! i) bs)"
+          using distinct_Complete_it prems(1) by simp
+        hence "distinct (items (bins (app_bins bs k (Complete_it k (items (bins bs ! k) ! i) bs)) ! k))"
+          using distinct_app_bins \<open>distinct (items (bins bs ! k))\<close> by blast
+
+        thm prems
+
+        have 0: "2 * card (UNIV_wf_kth_bin k) \<ge> Suc (card (set (items (bins (app_bins bs k (Complete_it k (items (bins bs ! k) ! i) bs)) ! k))) + i)"
+          sorry
+        have "Suc (length (items (bins (app_bins bs k (Complete_it k (items (bins bs ! k) ! i) bs)) ! k)) + i) > length (items (bins bs ! k)) + i"        
+          by (simp add: length_nth_bin_app_bins less_Suc_eq_le)
+        hence 1: "Suc (card (set (items (bins (app_bins bs k (Complete_it k (items (bins bs ! k) ! i) bs)) ! k))) + i) > card (set (items (bins bs ! k))) + i"
+          using distinct_card
+          by (metis \<open>distinct (items (bins (app_bins bs k (Complete_it k (items (bins bs ! k) ! i) bs)) ! k))\<close> \<open>distinct (items (bins bs ! k))\<close>)
+        show ?thesis
+          using 0 1 by simp
+      qed
+      sorry
+  qed
+  done
 (* while_option :: "('a \<Rightarrow> bool) \<Rightarrow> ('a \<Rightarrow> 'a) \<Rightarrow> 'a \<Rightarrow> 'a option"
    while :: "('a \<Rightarrow> bool) \<Rightarrow> ('a \<Rightarrow> 'a) \<Rightarrow> 'a \<Rightarrow> 'a" *)
 
@@ -160,24 +361,6 @@ qed
 
 declare \<pi>_it'.simps[simp del]
 
-subsection \<open>Bin lemmas\<close>
-
-lemma length_bins_app_bins[simp]:
-  "length (bins (app_bins bs k is)) = length (bins bs)"
-  unfolding app_bins_def by simp
-
-lemma length_nth_bin_app_bins:
-  "length (items (bins (app_bins bs k is) ! l)) \<ge> length (items (bins bs ! l))"
-  by (cases "k < length (bins bs)") (auto simp: nth_list_update app_bins_def app_bin_def)
-
-lemma length_nth_bin_app_bins_eq:
-  "k \<noteq> l \<Longrightarrow> length (items (bins (app_bins bs k is) ! l)) = length (items (bins bs ! l))"
-  by (cases "k < length (bins bs)") (auto simp: app_bins_def app_bin_def)
-
-lemma length_bins_Init_it[simp]:
-  "length (bins Init_it) = length inp + 1"
-  unfolding Init_it_def using length_bins_app_bins by force
-
 lemma length_bins_\<pi>_it'[simp]:
   "length (bins (\<pi>_it' k bs i)) = length (bins bs)"
   by (induction k bs i rule: \<pi>_it'_induct) auto
@@ -194,25 +377,6 @@ lemma length_nth_bin_\<pi>_it':
 lemma length_bins_\<I>_it[simp]:
   "length (bins (\<I>_it k)) = length (bins Init_it)"
   by (induction k) auto
-
-declare set_bin_def[simp]
-
-lemma app_bins_eq:
-  "set is \<subseteq> set_bin (bins bs ! k) \<Longrightarrow> app_bins bs k is = bs"
-  using filter_False unfolding app_bins_def app_bin_def by (auto simp: in_mono)
-
-lemma nth_app_bin:
-  "i < length (items b) \<Longrightarrow> items (app_bin b is) ! i = items b ! i"
-  unfolding app_bin_def by (simp add: nth_append)
-
-lemma nth_app_bins:
-  "k \<noteq> l \<Longrightarrow> bins (app_bins bs k is) ! l = bins bs ! l"
-  unfolding app_bins_def nth_app_bin by simp
-
-lemma kth_app_bins:
-  assumes "i < length (items (bins bs ! k))"
-  shows "items (bins (app_bins bs k is) ! k) ! i = items (bins bs ! k) ! i"
-  by (cases "k < length (bins bs)") (auto simp: app_bins_def nth_app_bin assms)
 
 lemma kth_\<pi>_it'_bins:
   assumes "j < length (items (bins bs ! l))"
@@ -240,135 +404,14 @@ proof standard
     by simp
 qed
 
-lemma set_bin_\<pi>_it'_eq:
-  "l < k \<Longrightarrow> set_bin (bins (\<pi>_it' k bs i) ! l) = set_bin (bins bs ! l)"
-  by (induction k bs i rule: \<pi>_it'_induct) (auto simp: app_bins_def nth_app_bins)
-
-lemma set_bin_upto_eq_set_bin:
-  "i \<ge> length (items b) \<Longrightarrow> set_bin_upto b i = set_bin b"
-  unfolding set_bin_upto_def set_bin_def by (auto, metis in_set_conv_nth less_le_trans)
-
 lemma set_bins_upto_k0_\<pi>_it'_eq:
   "k < length (bins bs) \<Longrightarrow> set_bins_upto (\<pi>_it k bs) k 0 = set_bins_upto bs k 0"
   unfolding set_bins_upto_def set_bin_upto_def \<pi>_it_def using set_bin_\<pi>_it'_eq by auto
 
-lemma set_bins_upto_empty:
-  "set_bins_upto bs 0 0 = {}"
-  unfolding set_bins_upto_def set_bin_upto_def by simp
 
-lemma set_bin_app_bin[simp]:
-  "set_bin (app_bin b is) = set_bin b \<union> set is"
-  unfolding app_bin_def by auto
-
-lemma set_bins_app_bins:
-  "k < length (bins bs) \<Longrightarrow> set_bins (app_bins bs k is) = set_bins bs \<union> set is"
-  unfolding set_bins_def app_bins_def using set_bin_app_bin
-  by (auto; smt Un_iff nth_list_update_eq nth_list_update_neq set_bin_app_bin set_bin_def)+
-
-lemma kth_bin_in_bins:
-  "k < length (bins bs) \<Longrightarrow> set_bin (bins bs ! k) \<subseteq> set_bins bs"
-  unfolding set_bins_def set_bins_upto_def set_bin_upto_def by blast
-
-lemma set_bins_upto_kth_nth_id:
-  assumes "l < length (bins bs)" "k \<le> l" "i < length (items (bins bs ! k))"
-  shows "set_bins_upto (app_bins bs l is) k i = set_bins_upto bs k i"
-  unfolding set_bins_upto_def set_bin_def set_bin_upto_def app_bins_def app_bin_def
-  using assms by (auto simp: nth_append nth_list_update, metis not_less)
-
-lemma set_bins_upto_sub_set_bins:
-  "k < length (bins bs) \<Longrightarrow> set_bins_upto bs k i \<subseteq> set_bins bs"
-  unfolding set_bins_def set_bins_upto_def set_bin_upto_def using less_trans by (auto, blast)
-
-lemma set_bins_upto_Suc_Un:
-  "i < length (items (bins bs ! k)) \<Longrightarrow> set_bins_upto bs k (i+1) = set_bins_upto bs k i \<union> { items (bins bs ! k) ! i }"
-  unfolding set_bins_upto_def set_bin_upto_def using less_Suc_eq by auto
-
-lemma set_bins_upto_Suc_eq:
-  "i \<ge> length (items (bins bs ! k)) \<Longrightarrow> set_bins_upto bs k (i+1) = set_bins_upto bs k i"
-  unfolding set_bins_upto_def set_bin_upto_def by auto
-
-lemma set_bins_bin_exists:
-  "x \<in> set_bins bs \<Longrightarrow> \<exists>k < length (bins bs). x \<in> set_bin (bins bs ! k)"
-  unfolding set_bins_def by blast
-
-lemma distinct_app_bin:
-  "distinct (items b) \<Longrightarrow> distinct is \<Longrightarrow> distinct (items (app_bin b is))"
-  unfolding app_bin_def by auto
-
-subsection \<open>Wellformed Bins\<close>
-
-definition wf_bin :: "nat \<Rightarrow> 'a bin \<Rightarrow> bool" where
-  "wf_bin k b \<longleftrightarrow> distinct (items b) \<and> (\<forall>x \<in> set (items b). wf_item x \<and> item_end x = k)"
-
-definition wf_bins :: "'a bins \<Rightarrow> bool" where
-  "wf_bins bs \<longleftrightarrow> (\<forall>k < length (bins bs). wf_bin k (bins bs ! k))"
-
-lemma wf_bins_impl_wf_items:
-  "wf_bins bs \<Longrightarrow> wf_items (set_bins bs)"
-  unfolding wf_bins_def wf_bin_def wf_items_def set_bins_def by auto
-
-lemma wf_bins_app_bins:
-  "wf_bins bs \<Longrightarrow> distinct xs \<Longrightarrow> \<forall>x \<in> set xs. wf_item x \<and> item_end x = k \<Longrightarrow> wf_bins (app_bins bs k xs)"
-  unfolding wf_bins_def wf_bin_def app_bins_def using set_bin_app_bin distinct_app_bin
-  by (cases "k < length (bins bs)") (auto simp: nth_list_update, blast+)
-
-lemma wf_bins_kth_bin:
-  "wf_bins bs \<Longrightarrow> k < length (bins bs) \<Longrightarrow> x \<in> set_bin (bins bs ! k) \<Longrightarrow> wf_item x \<and> item_end x = k"
-  using set_bin_def wf_bin_def wf_bins_def by blast
-
-lemma wf_bins_Init_it:
-  "wf_bins Init_it"
-proof -
-  let ?rs = "filter (\<lambda>r. rule_head r = \<SS>) rules"
-  let ?b0 = "Bin (map (\<lambda>r. init_item r 0) ?rs)"
-  let ?bs = "replicate (length inp + 1) (Bin [])"
-  have "wf_bin 0 ?b0"
-    unfolding wf_bin_def wf_item_def using valid_rules by (auto simp: init_item_def distinct_map inj_on_def)
-  moreover have "wf_bins (Bins ?bs)"
-    unfolding wf_bins_def wf_bin_def using less_Suc_eq_0_disj by force
-  ultimately show ?thesis
-    using wf_bins_app_bins unfolding wf_bin_def by (simp add: Init_it_def)
-qed
-
-lemma distinct_Scan_it:
-  "distinct (Scan_it k a x)"
-  unfolding Scan_it_def by simp
-
-lemma distinct_Predict_it:
-  "distinct (Predict_it k X)"
-  unfolding Predict_it_def using valid_rules by (auto simp: init_item_def rule_head_def distinct_map inj_on_def)
-
-lemma distinct_Complete_it:
-  "wf_bins bs \<Longrightarrow> item_origin y < length (bins bs) \<Longrightarrow> distinct (Complete_it k y bs)"
-  unfolding Complete_it_def wf_bins_def wf_bin_def by (auto simp: distinct_map inj_on_def inc_item_def item.expand)
-
-lemma wf_bins_Scan_it':
-  assumes "wf_bins bs" "k < length (bins bs)" "x \<in> set_bin (bins bs ! k)"
-  assumes "k < length inp" "next_symbol x \<noteq> None" "y = inc_item x (k+1)"
-  shows "wf_item y \<and> item_end y = k+1"
-  using assms wf_bins_kth_bin[OF assms(1-3)]
-  unfolding wf_item_def inc_item_def next_symbol_def is_complete_def item_rule_body_def
-  by (auto split: if_splits)
-
-lemma wf_bins_Scan_it:
-  assumes "wf_bins bs" "k < length (bins bs)" "x \<in> set_bin (bins bs ! k)"
-  assumes "k \<le> length inp" "next_symbol x \<noteq> None"
-  shows "\<forall>y \<in> set (Scan_it k a x). wf_item y \<and> item_end y = (k+1)" 
-  using wf_bins_Scan_it'[OF assms(1-3) _ assms(5)] 
-  by (metis List.list.set(1,2) Scan_it_def empty_iff insert_iff)
-
-lemma wf_bins_Predict_it:
-  assumes "wf_bins bs" "k < length (bins bs)" "k \<le> length inp"
-  shows "\<forall>y \<in> set (Predict_it k X). wf_item y \<and> item_end y = k"
-  using assms by (auto simp: Predict_it_def wf_item_def wf_bins_def wf_bin_def init_item_def valid_rules)
-
-lemma wf_bins_Complete_it:
-  assumes "wf_bins bs" "k < length (bins bs)" "y \<in> set_bin (bins bs ! k)"
-  shows "\<forall>x \<in> set (Complete_it k y bs). wf_item x \<and> item_end x = k"
-  using assms wf_bins_kth_bin[OF assms]
-  unfolding Complete_it_def wf_bins_def wf_bin_def wf_item_def inc_item_def next_symbol_def
-            is_complete_def item_rule_body_def
-  by (auto, metis le_less_trans, metis le_less_trans le_trans)
+lemma set_bin_\<pi>_it'_eq:
+  "l < k \<Longrightarrow> set_bin (bins (\<pi>_it' k bs i) ! l) = set_bin (bins bs ! l)"
+  by (induction k bs i rule: \<pi>_it'_induct) (auto simp: app_bins_def nth_app_bins)
 
 lemma wf_bins_\<pi>_it':
   "wf_bins bs \<Longrightarrow> k < length (bins bs) \<Longrightarrow> k \<le> length inp \<Longrightarrow> wf_bins (\<pi>_it' k bs i)"
@@ -985,7 +1028,7 @@ next
   case (Predict k bs i x a)
   let ?bs' = "app_bins bs k (Predict_it k a)"
   have "k \<ge> length inp \<or> \<not> inp!k = a"
-    using Predict.hyps(4) valid_inp is_terminal_def by force
+    using Predict.hyps(4) is_terminal_def valid_input by force
   have x: "x \<in> set_bin (bins bs ! k)"
     using Predict.hyps(1,2) by auto
   have len: "i < length (items (bins ?bs' ! k))"
